Minimal code for #209

examples/bug-reports/bug209.fst
@@ -1,53 +1,31 @@
+module Bug209
+
+(* Need a way to name the implicit t in the body *)
+
+val foo : #t:Type -> x:t -> Lemma (x = x)
+let foo t x = ()
+(* currently getting
+bug209.fst(4,0-59,0) : Error
+Expected a term of type "(t:Type -> x:t -> Lemma (unit))";
+got a function "(fun t x -> ())" (Curried function, but not total)
+ *)
+
+(* There are more ways to write this:
+   Currently type arguments are made implicit by default,
+   whether they are ticket or not *)
+
+val foo2 : t:Type -> x:t -> Lemma (x = x)
+let foo2 t x = ()
 (*
-   Copyright 2015 Chantal Keller and Catalin Hritcu, Microsoft Research and Inria
+bug209.fst(17,0-19,3) : Error
+Expected a term of type "(t:Type -> x:t -> Lemma (unit))";
+got a function "(fun t x -> ())" (Curried function, but not total)
+ *)
 
-   Licensed under the Apache License, Version 2.0 (the "License");
-   you may not use this file except in compliance with the License.
-   You may obtain a copy of the License at
-
-       http://www.apache.org/licenses/LICENSE-2.0
-
-   Unless required by applicable law or agreed to in writing, software
-   distributed under the License is distributed on an "AS IS" BASIS,
-   WITHOUT WARRANTIES OR CONDITIONS OF ANY KIND, either express or implied.
-   See the License for the specific language governing permissions and
-   limitations under the License.
-*)
-
-
-module Wf
-
-
-type acc (a:Type) (r:(a -> a -> Type)) (x:a) : Type =
-  | AccIntro : (y:a -> r y x -> Tot (acc a r y)) -> acc a r x
-
-type well_founded (a:Type) (r:(a -> a -> Type)) = x:a -> acc a r x
-
-val acc_inv : r:('a -> 'a -> Type) -> x:'a -> a:(acc 'a r x) ->
-              Tot (e:(y:'a -> r y x -> Tot (acc 'a r y)){e << a})
-let acc_inv x a = match a with | AccIntro z h1 -> h1
-
-assume val axiom1 : a:Type -> b:Type -> f:(a -> Tot b) -> x:a ->
-                    Lemma (f x << f)
-
-(* Can't prove it is total : I know that [acc_inv x a << a]
-   but from this I cannot deduce [acc_inv x a y h << a] *)
-val fix_F : #aa:Type -> #r:(aa -> aa -> Type) -> #p:(aa -> Type) ->
-            (x:aa -> (y:aa -> r y x -> Tot (p y)) -> Tot (p x)) ->
-            x:aa -> a:(acc aa r x) -> Tot (p x) (decreases a)
+val foo3 : x:'a -> Lemma (x = x)
+let foo3 t x = ()
 (*
-val fix_F : r:('a -> 'a -> Type) -> p:('a -> Type) ->
-            (x:'a -> (y:'a -> r y x -> p y) -> p x) ->
-            x:'a -> acc 'a r x -> p x
-*)
-let rec fix_F #aa #r #p f x a =
-  f x (fun y h ->
-(*
-         axiom1 a (r y x -> Tot (acc a r y)) (acc_inv x a) y;
-         axiom1 (acc_inv x a y) h;
-*)
-         fix_F #aa #r #p f y (acc_inv x a y h))
-
-val fix : r:('a -> 'a -> Type) -> well_founded 'a r -> p:('a -> Type) ->
-          (x:'a -> (y:'a -> r y x -> p y) -> p x) -> x:'a -> p x
-let fix rwf f x = fix_F f x (rwf x)
+bug209.fst(28,0-34,0) : Error
+Expected a term of type "('a:Type -> x:'a -> Lemma (unit))";
+got a function "(fun t x -> ())" (Curried function, but not total)
+ *)
